backends/lean/Aeneas/Std/Slice.lean
@@ -100,7 +100,7 @@ theorem Slice.getElem!_Usize_eq {α : Type u} [Inhabited α] (v : Slice α) (i :
 @[expose] def Slice.set {α : Type u} (v: Slice α) (i: Usize) (x: α) : Slice α :=
   Slice.setAtNat v i.val x
 
-def Slice.set_opt {α : Type u} (v: Slice α) (i: Usize) (x: Option α) : Slice α :=
+@[expose] def Slice.set_opt {α : Type u} (v: Slice α) (i: Usize) (x: Option α) : Slice α :=
   .from (v.val.set_opt i.val x) (by have := v.property; simp [*])
 
 @[expose] def Slice.drop {α} (s : Slice α) (i : Usize) : Slice α :=
@@ -120,7 +120,7 @@ abbrev Slice.slice {α : Type u} [Inhabited α] (s : Slice α) (i j : Nat) : Lis
   | none => fail .arrayOutOfBounds
   | some x => ok x
 
-@[rust_fun "core::slice::{[@T]}::is_empty", simp]
+@[expose, rust_fun "core::slice::{[@T]}::is_empty", simp]
 def core.slice.Slice.is_empty {T : Type} (s : Slice T) : Result Bool := ok (s.length = 0)
 
 @[step]
@@ -258,7 +258,7 @@ theorem Slice.getElem_Nat_setAtNat_ne
   (v.setAtNat i x).val[j] = v.val[j] := by
   simp only [setAtNat]; grind
 
-def Slice.update {α : Type u} (v: Slice α) (i: Usize) (x: α) : Result (Slice α) :=
+@[expose] def Slice.update {α : Type u} (v: Slice α) (i: Usize) (x: α) : Result (Slice α) :=
   match v.val[i.val]? with
   | none => fail .arrayOutOfBounds
   | some _ =>
@@ -290,7 +290,7 @@ theorem Slice.update_index_eq α [Inhabited α] (x : Slice α) (i : Usize) (h : 
   x.set i (x.val[i.val]'h) = x := by
   simp only [Slice.eq_iff, set_val_eq, List.set_getElem_self]
 
-def Slice.subslice {α : Type u} (s : Slice α) (r : Range Usize) : Result (Slice α) :=
+@[expose] def Slice.subslice {α : Type u} (s : Slice α) (r : Range Usize) : Result (Slice α) :=
   -- TODO: not completely sure here
   if r.start.val < r.end.val ∧ r.end.val ≤ s.length then
     ok (.from ( s.val.slice r.start.val r.end.val)
@@ -312,7 +312,7 @@ theorem Slice.subslice_spec {α : Type u} [Inhabited α] (s : Slice α) (r : Ran
   simp only [List.getElem!_eq_getElem?_getD] at *
   apply this
 
-def Slice.update_subslice {α : Type u} (s : Slice α) (r : Range Usize) (ss : Slice α) : Result (Slice α) :=
+@[expose] def Slice.update_subslice {α : Type u} (s : Slice α) (r : Range Usize) (ss : Slice α) : Result (Slice α) :=
   -- TODO: not completely sure here
   if h: r.start.val < r.end.val ∧ r.end.val ≤ s.length ∧ ss.val.length = r.end.val - r.start.val then
     ok (.from ( s.val.setSlice! r.start.val ss.val) (by simp))
@@ -330,7 +330,7 @@ theorem Slice.update_subslice_spec {α : Type u} [Inhabited α] (a : Slice α) (
     spec_ok, *]
   simp_lists
 
-@[rust_fun "core::slice::{[@T]}::reverse" -canFail]
+@[expose, rust_fun "core::slice::{[@T]}::reverse" -canFail]
 def core.slice.Slice.reverse {T : Type} (s : Slice T) : Slice T :=
   .from (s.val.reverse) (by simp)
 
@@ -349,7 +349,7 @@ def core.slice.index.Slice.index
   (slice : Slice T) (i : I) : Result Output :=
   inst.index i slice
 
-@[rust_fun "core::slice::{[@T]}::get"]
+@[expose, rust_fun "core::slice::{[@T]}::get"]
 def core.slice.Slice.get
   {T I Output : Type} (inst : core.slice.index.SliceIndex I (Slice T) Output)
   (s : Slice T) (i : I) : Result (Option Output) :=
@@ -362,20 +362,20 @@ opaque core.slice.Slice.get_unchecked
   (s : Slice T) (i : I) : Result Output
   -- TODO: we need to model the heap to call `SliceIndexInst.get_unchecked`
 
-@[rust_fun "core::slice::{[@T]}::get_mut"]
+@[expose, rust_fun "core::slice::{[@T]}::get_mut"]
 def core.slice.Slice.get_mut
   {T I Output : Type} (inst : core.slice.index.SliceIndex I (Slice T) Output)
   (s : Slice T) (i : I) : Result ((Option Output) × (Option Output → Slice T)) :=
   inst.get_mut i s
 
-@[rust_fun "core::slice::index::{core::slice::index::SliceIndex<core::ops::range::Range<usize>, [@T], [@T]>}::get"]
+@[expose, rust_fun "core::slice::index::{core::slice::index::SliceIndex<core::ops::range::Range<usize>, [@T], [@T]>}::get"]
 def core.slice.index.SliceIndexRangeUsizeSlice.get {T : Type} (r : Range Usize) (s : Slice T) :
   Result (Option (Slice T)) :=
   if r.start ≤ r.end ∧ r.end ≤ s.length then
     ok (some (.from (s.val.slice r.start r.end) (by scalar_tac)))
   else ok none
 
-@[rust_fun "core::slice::index::{core::slice::index::SliceIndex<core::ops::range::Range<usize>, [@T], [@T]>}::get_mut"]
+@[expose, rust_fun "core::slice::index::{core::slice::index::SliceIndex<core::ops::range::Range<usize>, [@T], [@T]>}::get_mut"]
 def core.slice.index.SliceIndexRangeUsizeSlice.get_mut
   {T : Type} (r : Range Usize) (s : Slice T) : Result (Option (Slice T) × (Option (Slice T) → Slice T)) :=
   if r.start ≤ r.end ∧ r.end ≤ s.length then
@@ -389,13 +389,13 @@ def core.slice.index.SliceIndexRangeUsizeSlice.get_mut
           else s )
   else ok (none, fun _ => s)
 
-@[rust_fun "core::slice::index::{core::slice::index::SliceIndex<core::ops::range::Range<usize>, [@T], [@T]>}::get_unchecked"]
+@[expose, rust_fun "core::slice::index::{core::slice::index::SliceIndex<core::ops::range::Range<usize>, [@T], [@T]>}::get_unchecked"]
 def core.slice.index.SliceIndexRangeUsizeSlice.get_unchecked {T : Type} :
   Range Usize → ConstRawPtr (Slice T) → Result (ConstRawPtr (Slice T)) :=
   -- Don't know what the model should be - for now we always fail
   fun _ _ => fail .undef
 
-@[rust_fun "core::slice::index::{core::slice::index::SliceIndex<core::ops::range::Range<usize>, [@T], [@T]>}::get_unchecked_mut"]
+@[expose, rust_fun "core::slice::index::{core::slice::index::SliceIndex<core::ops::range::Range<usize>, [@T], [@T]>}::get_unchecked_mut"]
 def core.slice.index.SliceIndexRangeUsizeSlice.get_unchecked_mut {T : Type} :
   Range Usize → MutRawPtr (Slice T) → Result (MutRawPtr (Slice T)) :=
   -- Don't know what the model should be - for now we always fail
@@ -426,7 +426,7 @@ def core.slice.index.Slice.index_mut
   (s : Slice T) (i : I) : Result (Output × (Output → Slice T)) :=
   inst.index_mut i s
 
-@[reducible, expose, rust_trait_impl "core::slice::index::SliceIndex<core::ops::range::Range<usize>, [@T], [@T]>"]
+@[expose, reducible, rust_trait_impl "core::slice::index::SliceIndex<core::ops::range::Range<usize>, [@T], [@T]>"]
 def core.slice.index.SliceIndexRangeUsizeSlice (T : Type) :
   core.slice.index.SliceIndex (Range Usize) (Slice T) (Slice T) := {
   get := core.slice.index.SliceIndexRangeUsizeSlice.get
@@ -437,14 +437,14 @@ def core.slice.index.SliceIndexRangeUsizeSlice (T : Type) :
   index_mut := core.slice.index.SliceIndexRangeUsizeSlice.index_mut
 }
 
-@[rust_fun "core::slice::index::{core::slice::index::SliceIndex<core::ops::range::RangeTo<usize>, [@T], [@T]>}::get"]
+@[expose, rust_fun "core::slice::index::{core::slice::index::SliceIndex<core::ops::range::RangeTo<usize>, [@T], [@T]>}::get"]
 def core.slice.index.SliceIndexRangeToUsizeSlice.get
   {T : Type} (r : core.ops.range.RangeTo Usize) (s : Slice T) : Result (Option (Slice T)) :=
   if r.end ≤ s.length then
     ok (some (.from (s.val.slice 0 r.end) (by scalar_tac)))
   else ok none
 
-@[rust_fun "core::slice::index::{core::slice::index::SliceIndex<core::ops::range::RangeTo<usize>, [@T], [@T]>}::get_mut"]
+@[expose, rust_fun "core::slice::index::{core::slice::index::SliceIndex<core::ops::range::RangeTo<usize>, [@T], [@T]>}::get_mut"]
 def core.slice.index.SliceIndexRangeToUsizeSlice.get_mut
   {T : Type} (r : core.ops.range.RangeTo Usize) (s : Slice T) :
   Result ((Option (Slice T)) × (Option (Slice T) → Slice T)) :=
@@ -459,13 +459,13 @@ def core.slice.index.SliceIndexRangeToUsizeSlice.get_mut
           else s )
   else ok (none, fun _ => s)
 
-@[rust_fun "core::slice::index::{core::slice::index::SliceIndex<core::ops::range::RangeTo<usize>, [@T], [@T]>}::get_unchecked"]
+@[expose, rust_fun "core::slice::index::{core::slice::index::SliceIndex<core::ops::range::RangeTo<usize>, [@T], [@T]>}::get_unchecked"]
 def core.slice.index.SliceIndexRangeToUsizeSlice.get_unchecked
   {T : Type} (_ : core.ops.range.RangeTo Usize) (_ : ConstRawPtr (Slice T)) : Result (ConstRawPtr (Slice T)) :=
   -- TODO: update once we make the model of computation more stateful (for now we just fail)
   fail .undef
 
-@[rust_fun "core::slice::index::{core::slice::index::SliceIndex<core::ops::range::RangeTo<usize>, [@T], [@T]>}::get_unchecked_mut"]
+@[expose, rust_fun "core::slice::index::{core::slice::index::SliceIndex<core::ops::range::RangeTo<usize>, [@T], [@T]>}::get_unchecked_mut"]
 def core.slice.index.SliceIndexRangeToUsizeSlice.get_unchecked_mut
   {T : Type} (_ : core.ops.range.RangeTo Usize) (_ : MutRawPtr (Slice T)) :
   Result (MutRawPtr (Slice T)) :=
@@ -492,7 +492,7 @@ def core.slice.index.SliceIndexRangeToUsizeSlice.index_mut
         fun s' => .from (List.setSlice! s.val 0 s'.val) (by simp))
   else fail .panic
 
-@[reducible, expose, rust_trait_impl "core::slice::index::SliceIndex<core::ops::range::RangeTo<usize>, [@T], [@T]>"]
+@[expose, reducible, rust_trait_impl "core::slice::index::SliceIndex<core::ops::range::RangeTo<usize>, [@T], [@T]>"]
 def core.slice.index.SliceIndexRangeToUsizeSlice (T : Type) :
   core.slice.index.SliceIndex (core.ops.range.RangeTo Usize) (Slice T) (Slice
   T) := {
@@ -513,7 +513,7 @@ abbrev core.slice.index.SliceIndexRangeFullSlice.get
   {T : Type} (_ : core.ops.range.RangeFull) (s : Slice T) : Result (Option (Slice T)) :=
   ok (some s)
 
-@[simp, step_simps, rust_fun "core::slice::index::{core::slice::index::SliceIndex<core::ops::range::RangeFull, [@T], [@T]>}::get_mut"]
+@[expose, simp, step_simps, rust_fun "core::slice::index::{core::slice::index::SliceIndex<core::ops::range::RangeFull, [@T], [@T]>}::get_mut"]
 def core.slice.index.SliceIndexRangeFullSlice.get_mut
   {T : Type} (_ : core.ops.range.RangeFull) (s : Slice T) :
   Result (Option (Slice T) × (Option (Slice T) → Slice T)) :=
@@ -531,18 +531,18 @@ opaque core.slice.index.SliceIndexRangeFullSlice.get_unchecked_mut
   Result (MutRawPtr (Slice T)) :=
   fail .undef -- TODO: not sure what it should be
 
-@[simp, step_simps, rust_fun "core::slice::index::{core::slice::index::SliceIndex<core::ops::range::RangeFull, [@T], [@T]>}::index"]
+@[expose, simp, step_simps, rust_fun "core::slice::index::{core::slice::index::SliceIndex<core::ops::range::RangeFull, [@T], [@T]>}::index"]
 def core.slice.index.SliceIndexRangeFullSlice.index
   {T : Type} (_ : core.ops.range.RangeFull) (s : Slice T) : Result (Slice T) :=
   ok s
 
-@[simp, step_simps, rust_fun "core::slice::index::{core::slice::index::SliceIndex<core::ops::range::RangeFull, [@T], [@T]>}::index_mut"]
+@[expose, simp, step_simps, rust_fun "core::slice::index::{core::slice::index::SliceIndex<core::ops::range::RangeFull, [@T], [@T]>}::index_mut"]
 def core.slice.index.SliceIndexRangeFullSlice.index_mut
   {T : Type} (_ : core.ops.range.RangeFull) (s : Slice T) :
   Result (Slice T × (Slice T → Slice T)) :=
   ok (s, fun updated => updated)
 
-@[reducible, rust_trait_impl "core::slice::index::SliceIndex<core::ops::range::RangeFull, [@T], [@T]>"]
+@[expose, reducible, rust_trait_impl "core::slice::index::SliceIndex<core::ops::range::RangeFull, [@T], [@T]>"]
 def core.slice.index.SliceIndexRangeFullSlice (T : Type) :
   core.slice.index.SliceIndex core.ops.range.RangeFull (Slice T) (Slice T) := {
   get := core.slice.index.SliceIndexRangeFullSlice.get
@@ -578,13 +578,13 @@ abbrev core.slice.index.Usize.get_mut
   {T : Type} (i : Usize) (s : Slice T) : Result (Option T × (Option T → Slice T)) :=
   ok (s[i]?, s.set_opt i)
 
-@[rust_fun "core::slice::index::{core::slice::index::SliceIndex<usize, [@T], @T>}::get_unchecked"]
+@[expose, rust_fun "core::slice::index::{core::slice::index::SliceIndex<usize, [@T], @T>}::get_unchecked"]
 def core.slice.index.Usize.get_unchecked
   {T : Type} : Usize → ConstRawPtr (Slice T) → Result (ConstRawPtr T) :=
   -- We don't have a model for now
   fun _ _ => fail .undef
 
-@[rust_fun "core::slice::index::{core::slice::index::SliceIndex<usize, [@T], @T>}::get_unchecked_mut"]
+@[expose, rust_fun "core::slice::index::{core::slice::index::SliceIndex<usize, [@T], @T>}::get_unchecked_mut"]
 def core.slice.index.Usize.get_unchecked_mut
   {T : Type} : Usize → MutRawPtr (Slice T) → Result (MutRawPtr T) :=
   -- We don't have a model for now
@@ -599,7 +599,7 @@ abbrev core.slice.index.Usize.index_mut {T : Type}
   (i : Usize) (s : Slice T) : Result (T × (T → (Slice T))) :=
   Slice.index_mut_usize s i
 
-@[reducible, expose, rust_trait_impl "core::slice::index::SliceIndex<usize, [@T], @T>"]
+@[expose, reducible, rust_trait_impl "core::slice::index::SliceIndex<usize, [@T], @T>"]
 def core.slice.index.SliceIndexUsizeSlice (T : Type) :
   core.slice.index.SliceIndex Usize (Slice T) T := {
   get := core.slice.index.Usize.get
@@ -617,19 +617,19 @@ axiom core.slice.Slice.get_unchecked_SliceIndexUsizeSlice_spec {T s i} [Inhabite
   ⦃ x => x = s[i] ⦄
   -- TODO: awaiting a full definition for `core.slice.Slice.get_unchecked`
 
-@[rust_fun "core::slice::{[@T]}::copy_from_slice"]
+@[expose, rust_fun "core::slice::{[@T]}::copy_from_slice"]
 def core.slice.Slice.copy_from_slice {T : Type} (_ : core.marker.Copy T)
   (s : Slice T) (src: Slice T) : Result (Slice T) :=
   if s.len = src.len then ok src
   else fail panic
 
-@[rust_fun "core::slice::index::{core::slice::index::SliceIndex<core::ops::range::RangeFrom<usize>, [@T], [@T]>}::get"]
+@[expose, rust_fun "core::slice::index::{core::slice::index::SliceIndex<core::ops::range::RangeFrom<usize>, [@T], [@T]>}::get"]
 def core.slice.index.SliceIndexRangeFromUsizeSlice.get {T : Type} (r : core.ops.range.RangeFrom Usize) (s : Slice T) : Result (Option (Slice T)) :=
   if  r.start ≤ s.length then
     ok (some (s.drop r.start))
   else ok none
 
-@[rust_fun "core::slice::index::{core::slice::index::SliceIndex<core::ops::range::RangeFrom<usize>, [@T], [@T]>}::get_mut"]
+@[expose, rust_fun "core::slice::index::{core::slice::index::SliceIndex<core::ops::range::RangeFrom<usize>, [@T], [@T]>}::get_mut"]
 def core.slice.index.SliceIndexRangeFromUsizeSlice.get_mut
   {T : Type} (r : core.ops.range.RangeFrom Usize) (s : Slice T) :
   Result ((Option (Slice T)) × (Option (Slice T) → Slice T)) :=
@@ -643,13 +643,13 @@ def core.slice.index.SliceIndexRangeFromUsizeSlice.get_mut
           else s)
   else ok (none, fun _ => s)
 
-@[rust_fun "core::slice::index::{core::slice::index::SliceIndex<core::ops::range::RangeFrom<usize>, [@T], [@T]>}::get_unchecked"]
+@[expose, rust_fun "core::slice::index::{core::slice::index::SliceIndex<core::ops::range::RangeFrom<usize>, [@T], [@T]>}::get_unchecked"]
 def core.slice.index.SliceIndexRangeFromUsizeSlice.get_unchecked {T : Type} :
   core.ops.range.RangeFrom Usize → ConstRawPtr (Slice T) → Result (ConstRawPtr (Slice T)) :=
   -- We don't have a model for now
   fun _ _ => fail .undef
 
-@[rust_fun "core::slice::index::{core::slice::index::SliceIndex<core::ops::range::RangeFrom<usize>, [@T], [@T]>}::get_unchecked_mut"]
+@[expose, rust_fun "core::slice::index::{core::slice::index::SliceIndex<core::ops::range::RangeFrom<usize>, [@T], [@T]>}::get_unchecked_mut"]
 def core.slice.index.SliceIndexRangeFromUsizeSlice.get_unchecked_mut {T : Type} :
   core.ops.range.RangeFrom Usize → MutRawPtr (Slice T) → Result (MutRawPtr (Slice T)) :=
   -- We don't have a model for now
@@ -683,7 +683,7 @@ theorem _SliceIndexRangeFromUsizeSlice.index_mut.test {T} (s : Slice T) (r : cor
   unfold core.slice.index.SliceIndexRangeFromUsizeSlice.index_mut
   simp [h]
 
-@[reducible, expose, rust_trait_impl "core::slice::index::SliceIndex<core::ops::range::RangeFrom<usize>, [@T], [@T]>"]
+@[expose, reducible, rust_trait_impl "core::slice::index::SliceIndex<core::ops::range::RangeFrom<usize>, [@T], [@T]>"]
 def core.slice.index.SliceIndexRangeFromUsizeSlice (T : Type) :
   core.slice.index.SliceIndex (core.ops.range.RangeFrom Usize) (Slice T) (Slice T) := {
   get := core.slice.index.SliceIndexRangeFromUsizeSlice.get
@@ -698,7 +698,7 @@ def core.slice.index.SliceIndexRangeFromUsizeSlice (T : Type) :
 }
 
 /-- Small helper (this function doesn't model a specific Rust function) -/
-def Slice.clone {T : Type} (clone : T → Result T) (s : Slice T) : Result (Slice T) := do
+@[expose] def Slice.clone {T : Type} (clone : T → Result T) (s : Slice T) : Result (Slice T) := do
   let s' ← List.clone clone s.val
   ok (.from s' (by simp))
 
@@ -715,7 +715,7 @@ theorem Slice.clone_spec {T : Type} {clone : T → Result T} {s : Slice T} (h : 
   have ⟨ _, h ⟩ := spec_imp_exists (List.clone_spec h)
   simp [h]
 
-@[rust_fun "core::slice::{[@T]}::split_at"]
+@[expose, rust_fun "core::slice::{[@T]}::split_at"]
 def core.slice.Slice.split_at {T : Type} (s : Slice T) (n : Usize) :
   Result ((Slice T) × (Slice T)) :=
   if h0 : n ≤ s.length then
@@ -726,7 +726,7 @@ def core.slice.Slice.split_at {T : Type} (s : Slice T) (n : Usize) :
     ok (s0, s1)
   else fail .panic
 
-@[rust_fun "core::slice::{[@T]}::split_at_mut"]
+@[expose, rust_fun "core::slice::{[@T]}::split_at_mut"]
 def core.slice.Slice.split_at_mut {T : Type} (s : Slice T) (n : Usize) :
   Result (((Slice T) × (Slice T)) × (((Slice T) × (Slice T)) → Slice T)) :=
   if h0 : n ≤ s.length then
@@ -786,7 +786,7 @@ theorem core.slice.Slice.split_at_mut.spec {T : Type} (s : Slice T) (n : Usize)
       simp [Slice.length, List.splitAt_eq] at *
       exact ⟨by scalar_tac, by scalar_tac⟩
 
-@[rust_fun "core::slice::{[@T]}::swap"]
+@[expose, rust_fun "core::slice::{[@T]}::swap"]
 def core.slice.Slice.swap {T : Type} (s : Slice T) (a b : Usize) : Result (Slice T) := do
   let av ← Slice.index_usize s a
   let bv ← Slice.index_usize s b
@@ -1018,7 +1018,7 @@ theorem core.slice.Slice.copy_from_slice.step_spec (copyInst : core.marker.Copy 
   simp only [Slice.len]
   simp [h]
 
-def Slice.mapM  {α β} (f : α → Result β) (x : Slice α) : Result (Slice β) :=
+@[expose] def Slice.mapM  {α β} (f : α → Result β) (x : Slice α) : Result (Slice β) :=
   do let ⟨l, p⟩ ← List.mapM_with_length f x.val
      ok (.from l (by grind))
 
@@ -1045,7 +1045,7 @@ theorem Slice.mapM_spec {α β} {f : α → Result β} {s : Slice α} {post : Na
 
 /-- Model for `<[T]>::fill(v)`: returns a slice of the same length where every
     element is obtained by calling `clone(v)`. Mirrors Rust stdlib. -/
-@[rust_fun "core::slice::{[@T]}::fill"]
+@[expose, rust_fun "core::slice::{[@T]}::fill"]
 def core.slice.Slice.fill {T : Type} (cloneInst : core.clone.Clone T)
     (s : Slice T) (v : T) : Result (Slice T) :=
   do let ⟨l, p⟩ ← List.mapM_with_length (fun _ => cloneInst.clone v) s.val
