backends/lean/Aeneas/Std/Core/Default.lean
@@ -9,7 +9,7 @@ namespace Aeneas.Std
 structure core.default.Default (Self : Type u) where
   default : Result Self
 
-@[rust_fun "core::default::{core::default::Default<bool>}::default"]
+@[expose, rust_fun "core::default::{core::default::Default<bool>}::default"]
 def core.default.DefaultBool.default : Result Bool := .ok false
 
 end Aeneas.Std
