backends/lean/Aeneas/Std/Scalar/Bitwise.lean
@@ -16,65 +16,65 @@ open Result Error Arith ScalarElab WP
 /-!
 Bit shifts
 -/
-def UScalar.shiftLeft {ty : UScalarTy} (x : UScalar ty) (s : Nat) :
+@[expose] def UScalar.shiftLeft {ty : UScalarTy} (x : UScalar ty) (s : Nat) :
   Result (UScalar ty) :=
   if s < ty.numBits then
     ok ⟨ x.bv.shiftLeft s ⟩
   else fail .integerOverflow
 
-def UScalar.shiftRight {ty : UScalarTy} (x : UScalar ty) (s : Nat) :
+@[expose] def UScalar.shiftRight {ty : UScalarTy} (x : UScalar ty) (s : Nat) :
   Result (UScalar ty) :=
   if s < ty.numBits then
     ok ⟨ x.bv.ushiftRight s ⟩
   else fail .integerOverflow
 
-def UScalar.shiftLeft_UScalar {ty tys} (x : UScalar ty) (s : UScalar tys) :
+@[expose] def UScalar.shiftLeft_UScalar {ty tys} (x : UScalar ty) (s : UScalar tys) :
   Result (UScalar ty) :=
   x.shiftLeft s.val
 
-def UScalar.shiftRight_UScalar {ty tys} (x : UScalar ty) (s : UScalar tys) :
+@[expose] def UScalar.shiftRight_UScalar {ty tys} (x : UScalar ty) (s : UScalar tys) :
   Result (UScalar ty) :=
   x.shiftRight s.val
 
-def UScalar.shiftLeft_IScalar {ty tys} (x : UScalar ty) (s : IScalar tys) :
+@[expose] def UScalar.shiftLeft_IScalar {ty tys} (x : UScalar ty) (s : IScalar tys) :
   Result (UScalar ty) :=
   if s.val ≥ 0 then
     x.shiftLeft s.toNat
   else fail .integerOverflow
 
-def UScalar.shiftRight_IScalar {ty tys} (x : UScalar ty) (s : IScalar tys) :
+@[expose] def UScalar.shiftRight_IScalar {ty tys} (x : UScalar ty) (s : IScalar tys) :
   Result (UScalar ty) :=
   if s.val ≥ 0 then
     x.shiftRight s.toNat
   else fail .integerOverflow
 
-def IScalar.shiftLeft {ty : IScalarTy} (x : IScalar ty) (s : Nat) :
+@[expose] def IScalar.shiftLeft {ty : IScalarTy} (x : IScalar ty) (s : Nat) :
   Result (IScalar ty) :=
   if s < ty.numBits then
     ok ⟨ x.bv.shiftLeft s ⟩
   else fail .integerOverflow
 
-def IScalar.shiftRight {ty : IScalarTy} (x : IScalar ty) (s : Nat) :
+@[expose] def IScalar.shiftRight {ty : IScalarTy} (x : IScalar ty) (s : Nat) :
   Result (IScalar ty) :=
   if s < ty.numBits then
     ok ⟨ x.bv.sshiftRight s ⟩
   else fail .integerOverflow
 
-def IScalar.shiftLeft_UScalar {ty tys} (x : IScalar ty) (s : UScalar tys) :
+@[expose] def IScalar.shiftLeft_UScalar {ty tys} (x : IScalar ty) (s : UScalar tys) :
   Result (IScalar ty) :=
   x.shiftLeft s.val
 
-def IScalar.shiftRight_UScalar {ty tys} (x : IScalar ty) (s : UScalar tys) :
+@[expose] def IScalar.shiftRight_UScalar {ty tys} (x : IScalar ty) (s : UScalar tys) :
   Result (IScalar ty) :=
   x.shiftRight s.val
 
-def IScalar.shiftLeft_IScalar {ty tys} (x : IScalar ty) (s : IScalar tys) :
+@[expose] def IScalar.shiftLeft_IScalar {ty tys} (x : IScalar ty) (s : IScalar tys) :
   Result (IScalar ty) :=
   if s.val ≥ 0 then
     x.shiftLeft s.toNat
   else fail .integerOverflow
 
-def IScalar.shiftRight_IScalar {ty tys} (x : IScalar ty) (s : IScalar tys) :
+@[expose] def IScalar.shiftRight_IScalar {ty tys} (x : IScalar ty) (s : IScalar tys) :
   Result (IScalar ty) :=
   if s.val ≥ 0 then
     x.shiftRight s.toNat
@@ -146,9 +146,9 @@ instance {ty} : HXor (IScalar ty) (IScalar ty) (IScalar ty) where
 /-!
 Not
 -/
-def UScalar.not {ty} (x : UScalar ty) : UScalar ty := ⟨ ~~~x.bv ⟩
+@[expose] def UScalar.not {ty} (x : UScalar ty) : UScalar ty := ⟨ ~~~x.bv ⟩
 
-def IScalar.not {ty} (x : IScalar ty) : IScalar ty := ⟨ ~~~x.bv ⟩
+@[expose] def IScalar.not {ty} (x : IScalar ty) : IScalar ty := ⟨ ~~~x.bv ⟩
 
 instance {ty} : Complement (UScalar ty) where
   complement x := UScalar.not x
