backends/lean/Aeneas/Std/Scalar/Default.lean
@@ -12,13 +12,13 @@ open Result ScalarElab
 /- [core::default::{core::default::Default for u32}::default]:
    Source: '/rustc/library/core/src/default.rs', lines 156:12-156:30
    Name pattern: [core::default::{core::default::Default<u32>}::default] -/
-uscalar @[simp, scalar_tac_simps] def core.default.Default'S.default : «%S» := ⟨ 0, by scalar_tac ⟩
-iscalar @[simp, scalar_tac_simps] def core.default.Default'S.default : «%S» := ⟨ 0, by scalar_tac ⟩
+uscalar @[expose, simp, scalar_tac_simps] def core.default.Default'S.default : «%S» := ⟨ 0, by scalar_tac ⟩
+iscalar @[expose, simp, scalar_tac_simps] def core.default.Default'S.default : «%S» := ⟨ 0, by scalar_tac ⟩
 
 /- Trait implementation: [core::default::{core::default::Default for u32}#7]
    Source: '/rustc/library/core/src/default.rs', lines 153:8-153:27
    Name pattern: [core::default::Default<u32>] -/
-scalar @[reducible] def core.default.Default'S : core.default.Default «%S» := {
+scalar @[expose, reducible] def core.default.Default'S : core.default.Default «%S» := {
   default := ok core.default.Default'S.default }
 
 end Aeneas.Std
