backends/lean/Aeneas/Std/Scalar/Ops/Sub.lean
@@ -14,17 +14,17 @@ open Result Error Arith ScalarElab WP
 # Subtraction: Definitions
 -/
 
-def UScalar.sub {ty : UScalarTy} (x y : UScalar ty) : Result (UScalar ty) :=
+@[expose] def UScalar.sub {ty : UScalarTy} (x y : UScalar ty) : Result (UScalar ty) :=
   if x.val < y.val then fail .integerOverflow
   else ok ⟨ BitVec.ofNat _ (x.val - y.val) ⟩
 
-def IScalar.sub {ty : IScalarTy} (x y : IScalar ty) : Result (IScalar ty) :=
+@[expose] def IScalar.sub {ty : IScalarTy} (x y : IScalar ty) : Result (IScalar ty) :=
   IScalar.tryMk ty (x.val - y.val)
 
-def UScalar.try_sub {ty : UScalarTy} (x y : UScalar ty) : Option (UScalar ty) :=
+@[expose] def UScalar.try_sub {ty : UScalarTy} (x y : UScalar ty) : Option (UScalar ty) :=
   Option.ofResult (sub x y)
 
-def IScalar.try_sub {ty : IScalarTy} (x y : IScalar ty) : Option (IScalar ty) :=
+@[expose] def IScalar.try_sub {ty : IScalarTy} (x y : IScalar ty) : Option (IScalar ty) :=
   Option.ofResult (sub x y)
 
 instance {ty} : HSub (UScalar ty) (UScalar ty) (Result (UScalar ty)) where
